TestModels/SimpleTypes/SimpleEnumV2/src/SimpleEnumImpl.dfy
@@ -1,12 +1,10 @@
 include "../Model/SimpleTypesEnumV2Types.dfy"
 
-module SimpleEnumV2Impl refines AbstractSimpleTypesEnumV2Operations  {
+module SimpleEnumV2Impl refines AbstractSimpleTypesEnumV2Operations {
   datatype Config = Config
   type InternalConfig = Config
-  predicate ValidInternalConfig?(config: InternalConfig)
-  {true}
-  function ModifiesInternalConfig(config: InternalConfig) : set<object>
-  {{}}
+  predicate ValidInternalConfig?(config: InternalConfig) { true }
+  function ModifiesInternalConfig(config: InternalConfig): set<object> { {} }
   predicate GetEnumV2EnsuresPublicly(input: GetEnumV2Input, output: Result<GetEnumV2Output, Error>) {
     true
   }
@@ -19,49 +17,53 @@ module SimpleEnumV2Impl refines AbstractSimpleTypesEnumV2Operations  {
   predicate GetEnumV2ThirdKnownValueTestEnsuresPublicly(input: GetEnumV2Input, output: Result<GetEnumV2Output, Error>) {
     true
   }
-  method GetEnumV2 ( config: InternalConfig,  input: GetEnumV2Input )
-  returns (output: Result<GetEnumV2Output, Error>) {
+  method GetEnumV2(config: InternalConfig, input: GetEnumV2Input)
+    returns (output: Result<GetEnumV2Output, Error>)
+  {
     var res := GetEnumV2Output(value := input.value);
     return Success(res);
   }
 
   // Known value tests. See "Known value test" in TestModels' README.
-  method GetEnumV2FirstKnownValueTest ( config: InternalConfig,  input: GetEnumV2Input )
-  returns (output: Result<GetEnumV2Output, Error>) {
+  method GetEnumV2FirstKnownValueTest(config: InternalConfig, input: GetEnumV2Input)
+    returns (output: Result<GetEnumV2Output, Error>)
+  {
     expect input.value.Some?;
     expect input.value.value == FIRST;
 
     var res := GetEnumV2Output(value := input.value);
 
     expect res.value.Some?;
-    expect res.value.value == FIRST; 
+    expect res.value.value == FIRST;
 
     return Success(res);
   }
 
-  method GetEnumV2SecondKnownValueTest ( config: InternalConfig,  input: GetEnumV2Input )
-  returns (output: Result<GetEnumV2Output, Error>) {
+  method GetEnumV2SecondKnownValueTest(config: InternalConfig, input: GetEnumV2Input)
+    returns (output: Result<GetEnumV2Output, Error>)
+  {
     expect input.value.Some?;
     expect input.value.value == SECOND;
 
     var res := GetEnumV2Output(value := input.value);
 
     expect res.value.Some?;
-    expect res.value.value == SECOND; 
-    
+    expect res.value.value == SECOND;
+
     return Success(res);
   }
 
-  method GetEnumV2ThirdKnownValueTest ( config: InternalConfig,  input: GetEnumV2Input )
-  returns (output: Result<GetEnumV2Output, Error>) {
+  method GetEnumV2ThirdKnownValueTest(config: InternalConfig, input: GetEnumV2Input)
+    returns (output: Result<GetEnumV2Output, Error>)
+  {
     expect input.value.Some?;
     expect input.value.value == THIRD;
 
     var res := GetEnumV2Output(value := input.value);
 
     expect res.value.Some?;
-    expect res.value.value == THIRD; 
-    
+    expect res.value.value == THIRD;
+
     return Success(res);
   }
 }
